Add correct proofs for agree_on equivalence of combineenv

TransVal/transval.v
@@ -2,640 +2,13 @@ Require Import List Arith.
 Require Import IL Annotation AutoIndTac Bisim Exp MoreExp Coherence Fresh Util.
 Require Import SetOperations Sim Var.
 Require Import sexp smt nofun noGoto Terminates bitvec Crash freeVars.
-Require Import tvalTactics TUtil Guards.
+Require Import tvalTactics TUtil Guards crashProps termProps.
 
 Definition smtCheck (s:stmt) (t:stmt) :=
 smtAnd (translateStmt s source) (translateStmt t target).
 
 Definition combineEnv D (E1:onv val) E2 :=
 fun x => if [x ∈ D] then E1 x else E2 x.
-
-Lemma term_ssa_eval_agree L L' s D s' (E:onv val) (E':onv val)
- : ssa s D
-   -> noFun s
-   -> Terminates (L, E, s) (L', E', s')
-   -> agree_on eq (fst (getAnn D)) E E'.
-
-Proof.
-  intros.
-  general induction H1; invt ssa; try invt F.step;try invt noFun; simpl;
-  try reflexivity; isabsurd.
-  - exploit IHTerminates; [ | | reflexivity | reflexivity |]; eauto.
-   rewrite H7 in X; simpl in *. cset_tac; intuition.
-   hnf. hnf in X. intros.
-   unfold update in X. specialize (X x0).
-   assert (x0 ∈ D0 ++ {x; {}}) by (cset_tac; left; assumption).
-   specialize (X H10). decide (x === x0); eauto.
-    + rewrite  <- e0 in H8; exfalso; apply H4 ; assumption.
-  - exploit IHTerminates; [ | | reflexivity | reflexivity |]; eauto.
-    rewrite H9 in X; simpl in *. assumption.
-  - exploit IHTerminates; [| | reflexivity | reflexivity |]; eauto.
-    rewrite H10 in X; simpl in *; assumption.
-Qed.
-
-Lemma crash_ssa_eval_agree L L' s D s' (E:onv val) (E':onv val)
-: ssa s D
-  ->noFun s
-  -> Crash (L, E, s) (L', E', s')
-  -> agree_on eq (fst (getAnn (D))) E E'.
-
-Proof.
-  intros.
-  general induction H1; invt ssa; try invt F.step; try invt noFun; simpl;
-  try reflexivity; isabsurd.
-  - exploit IHCrash; [ | | reflexivity | reflexivity |]; eauto.
-    rewrite H7 in X; simpl in *; cset_tac; intuition.
-    hnf; hnf in X; intros.
-    unfold update in X; specialize (X x0).
-    assert (x0 ∈ D0 ++ {x; {}}) by (cset_tac; left; assumption).
-    specialize (X H10); decide (x === x0); eauto.
-    + rewrite <- e0 in H8; exfalso; eapply H4; assumption.
-  - exploit IHCrash; [ | | reflexivity | reflexivity |]; eauto.
-    rewrite H9 in X; eauto.
-  - exploit IHCrash; [ | | reflexivity | reflexivity |]; eauto.
-    rewrite H10 in X; eauto.
-Qed.
-
-Lemma terminates_impl_star2:
-  forall L E s L' Es s',
-    noFun s
-    -> Terminates (L, E ,s ) (L', Es, s')
-    -> (star2 F.step (L, E, s) nil (L', Es, s'))
-       /\ ((exists e, s' = stmtReturn e) \/ (exists f X, s' = stmtGoto f X)).
-
-Proof.
-intros.
-general induction H0; eauto.
--split; eauto; econstructor.
-- split; eauto; econstructor.
-- inversion H2; subst; try isabsurd.
-  + exploit (IHTerminates L' E' s'); try reflexivity.
-    * inversion H; subst; eauto.
-    * destruct X as [step X]; split.
-      { change (star2 F.step (L0, E0, stmtExp x e s) (filter_tau EvtTau nil) (L'0, Es, s'0)).
-        econstructor; eauto. destruct a; eauto; isabsurd. }
-      { destruct X; eauto. }
-  + exploit (IHTerminates L' E' s'); eauto.
-    * inversion H; subst; eauto.
-    * destruct X as [step X]; split.
-      { change (star2 F.step (L0, E0, stmtIf e s t)(filter_tau EvtTau nil) (L'0, Es, s'0)).
-        econstructor; eauto; destruct a; eauto; isabsurd. }
-      {destruct X; eauto. }
-Qed.
-
-Lemma terminates_impl_models :
-forall L s D E s' E',
-ssa  s D
--> noFun s
--> Terminates (L,E, s) (L, E', s')
-->  models (fun (f:pred) (x:vallst) => true)  E'  (translateStmt s source).
-
-Proof.
-intros.
-general induction H1; simpl.
-- assert (X: models (fun (_:pred) (_:vallst) => true) E0 (smtReturn e)).
-  + simpl. econstructor.
-  + case_eq (undef e); eauto; intros.
-    * simpl; split; eauto.
-      eapply (guard_true_if_eval); eauto.
-- case_eq (undefLift x); intros; simpl; eauto.
-  + split; eauto.
-       eapply (guardList_true_if_eval _ E0); eauto.
-- inv H; invt ssa; invt noFun; simpl in * |- *; subst.
-  + case_eq(undef e); intros; simpl; split; eauto.
-    * eapply (guard_true_if_eval _ E'0 e s v ); eauto.
-      eapply exp_eval_agree; eauto.
-      assert (A: agree_on eq (fst (getAnn (ann1 (D0, D') an))) E0 E'0).
-      { eapply (term_ssa_eval_agree L' L' (stmtExp x e s') _ s'0 _ _);
-        econstructor; eauto. }
-      { eapply (agree_on_incl  (bv:=Exp.freeVars e) (lv:=fst (getAnn (ann1 (D0, D') an)))); eauto. }
-    * split; eauto; subst.
-      assert (X1: exp_eval E'0 (Var x) = Some v).
-      { eapply (exp_eval_agree (E:= E0[x <- Some v])) ; eauto.
-        - simpl. eapply (agree_on_incl (bv:={x} ) (lv:= fst (getAnn an))); subst.
-          + eapply (term_ssa_eval_agree L' L' s' _ s'0 _ E'0); eauto.
-          + rewrite H11. unfold fst. cset_tac. right; rewrite H6; reflexivity.
-        - unfold exp_eval. unfold update. decide (x===x); eauto; isabsurd. }
-      assert (X2: exp_eval E'0 e = Some v).
-      { eapply exp_eval_agree; eauto.
-      assert (A: agree_on eq (fst (getAnn (ann1 (D0, D') an))) E0 E'0).
-        - eapply (term_ssa_eval_agree L' L' (stmtExp x e s') _ s'0 _ _);
-          econstructor; eauto.
-        - eapply (agree_on_incl  (bv:=Exp.freeVars e) (lv:=fst (getAnn (ann1 (D0, D') an)))); eauto. }
-      {  unfold evalSexp. rewrite X1; rewrite X2.
-         eapply  bvEq_equiv_eq. reflexivity. }
-    * assert (X1: exp_eval E'0 (Var x) = Some v).
-      { eapply (exp_eval_agree (E:= E0 [x <- Some v])) ; eauto.
-        - simpl. eapply (agree_on_incl (bv:={x} ) (lv:= fst (getAnn an))).
-          + eapply (term_ssa_eval_agree L' L' s' _ s'0 _ _); eauto.
-          + rewrite H11. unfold fst. cset_tac. right; rewrite H6; reflexivity.
-        - unfold exp_eval. unfold update. decide (x===x); eauto; isabsurd. }
-      assert (X2: exp_eval E'0 e = Some v).
-      { eapply exp_eval_agree; eauto.
-      assert (A: agree_on eq (fst (getAnn (ann1 (D0, D') an))) E0 E'0).
-        - eapply (term_ssa_eval_agree  L' L' (stmtExp x e s') _ s'0);
-          econstructor; eauto.
-        - eapply (agree_on_incl  (bv:=Exp.freeVars e) (lv:=fst (getAnn (ann1 (D0, D') an)))); eauto. }
-      {  unfold evalSexp. rewrite X1; rewrite X2.
-         eapply  bvEq_equiv_eq. reflexivity.  }
- + assert (X: models  (fun (_:pred) (_:vallst) => true) E'0 ( ite e (translateStmt s' source) (translateStmt b2 source))).
-    * simpl. unfold evalSexp.
-      assert (Exp.freeVars e ⊆ fst (getAnn (ann2 (D0, D') ans ant)))
-        by (hnf; intros; hnf in H7; specialize (H7 a); exact (H7 H4)).
-      assert (agree_on eq (fst (getAnn (ann2 (D0, D') ans ant))) E' E'0)
-        by ( eapply (term_ssa_eval_agree L' L' (stmtIf e s' b2) _ s'0 _ _); econstructor; eauto).
-      erewrite (exp_eval_agree (E:=E') (E':=E'0)); eauto. simpl. rewrite condTrue.
-      eapply IHTerminates; eauto.
-      eapply (agree_on_incl (bv:= Exp.freeVars e) (lv:= fst (getAnn (ann2 (D0, D') ans ant)))); eauto.
-    * case_eq (undef e); intros; eauto.
-      { simpl; split; eauto.
-        - eapply (guard_true_if_eval  (fun (_:pred) (_:vallst) => true) E'0 e _ v); eauto.
-          assert (Exp.freeVars e ⊆ fst (getAnn (ann2 (D0, D') ans ant)))
-            by (hnf; intros; hnf in H7; specialize (H7 a); hnf; cset_tac; simpl;  exact (H7 H5)).
-          assert (agree_on eq (fst (getAnn (ann2 (D0, D') ans ant))) E' E'0)
-            by ( eapply (term_ssa_eval_agree L' L' (stmtIf e s' b2) _ s'0 _ _); econstructor; eauto).
-          eapply (exp_eval_agree (E:=E') (E':=E'0)); eauto.
-          eapply (agree_on_incl (bv:= Exp.freeVars e) (lv:= fst (getAnn (ann2 (D0, D') ans ant)))); eauto.
-      }
- + assert (X: models  (fun (_:pred) (_:vallst) => true) E'0( ite e (translateStmt b1 source) (translateStmt s' source))).
-    * simpl. unfold evalSexp.
-      assert (Exp.freeVars e ⊆ fst (getAnn (ann2 (D0, D') ans ant)))
-        by (hnf; intros; hnf in H7; specialize (H7 a); exact (H7 H4)).
-      assert (agree_on eq (fst (getAnn (ann2 (D0, D') ans ant))) E' E'0)
-      by ( eapply (term_ssa_eval_agree L' L' (stmtIf e b1 s') _ s'0 _ _);econstructor;  eauto).
-      erewrite (exp_eval_agree (E:=E') (E':=E'0)); eauto. simpl. rewrite condFalse.
-      eapply IHTerminates; eauto.
-      eapply (agree_on_incl (bv:= Exp.freeVars e) (lv:= fst (getAnn (ann2 (D0, D') ans ant)))); eauto.
-    * case_eq (undef e); intros; eauto.
-      { simpl; split; eauto.
-        - eapply (guard_true_if_eval  (fun (_:pred) (_:vallst) => true) E'0 e _ v); eauto.
-          + assert (Exp.freeVars e ⊆ fst (getAnn (ann2 (D0, D') ans ant)))
-              by (hnf; intros; hnf in H7; specialize (H7 a); hnf; cset_tac; simpl;  exact (H7 H5)).
-            assert (agree_on eq (fst (getAnn (ann2 (D0, D') ans ant))) E' E'0)
-              by ( eapply (term_ssa_eval_agree L' L' (stmtIf e b1 s') _ s'0 _ _); econstructor; eauto).
-            eapply (exp_eval_agree (E:=E') (E':=E'0)); eauto.
-            eapply (agree_on_incl (bv:= Exp.freeVars e) (lv:= fst (getAnn (ann2 (D0, D') ans ant)))); eauto.
-      }
- + specialize (H0 l Y); isabsurd.
-Qed.
-
-Lemma undef_models:
-forall F E e g,
-(forall x, x ∈ Exp.freeVars e -> exists v, E x = Some v)
--> undef e =Some g
--> exp_eval E e = None
--> ~ models F E g.
-
-Proof.
-intros;  hnf;  intros.
-general induction e; simpl in *; try isabsurd.
-- monad_inv H1.
-  + specialize (IHe F E g H H0 H3 H2); eauto.
-  + destruct u; isabsurd.
-- destructBin b; monad_inv H1; try isabsurd.
-  + case_eq (undef e1); case_eq (undef e2); intros;
-    rewrite H4 in H0; rewrite H1 in H0; simpl in H0; inversion H0;
-    rewrite <- H6 in H2; simpl in H2; try destruct H2.
-    * eapply (IHe1 F E s0); eauto.
-      intros. cset_tac. specialize (H x). destruct H; eauto.
-    * eapply (IHe1 F E s); eauto.
-      intros; cset_tac; specialize (H x); destruct H; eauto.
-    * pose proof (noguard_impl_eval  E e1).
-      destruct H5; isabsurd; eauto.
-      intros; cset_tac; destruct (H x); eauto.
-  + case_eq (undef e1); case_eq (undef e2); intros;
-    rewrite H4 in H0; rewrite H3 in H0; simpl in H0; inversion H0;
-    rewrite <- H6 in H2; simpl in H2; try destruct H2.
-    * eapply (IHe2 F E s); eauto.
-      intros; cset_tac. destruct (H x0); eauto.
-    * pose proof (noguard_impl_eval E e2).
-      destruct H5; isabsurd; eauto.
-      intros; cset_tac. destruct (H x0); eauto.
-    * eapply (IHe2 F E s); eauto.
-      intros; cset_tac. destruct (H x0); eauto.
-  +  case_eq (undef e1); case_eq (undef e2); intros;
-    rewrite H4 in H0; rewrite H1 in H0; simpl in H0; inversion H0;
-    rewrite <- H6 in H2; simpl in H2; try destruct H2.
-     * eapply (IHe1 F E s0); eauto.
-       intros; cset_tac. destruct (H x); eauto.
-     * eapply (IHe1 F E s); eauto.
-       intros; cset_tac; destruct (H x); eauto.
-     * pose proof (noguard_impl_eval E e1).
-       destruct H5; eauto; isabsurd.
-       intros; cset_tac; destruct (H x); eauto.
-  + case_eq (undef e1); case_eq (undef e2); intros;
-    rewrite H4 in H0; rewrite H3 in H0; simpl in H0; inversion H0;
-    rewrite <- H6 in H2; simpl in H2; try destruct H2.
-    * eapply (IHe2 F E s); eauto.
-      intros; cset_tac. destruct (H x0); eauto.
-    * pose proof (noguard_impl_eval E e2).
-      destruct H5; eauto; isabsurd.
-      intros; cset_tac. destruct (H x0); eauto.
-    * eapply (IHe2 F E s); eauto.
-      intros; cset_tac. destruct (H x0); eauto.
-  + case_eq (undef e1); case_eq (undef e2); intros;
-    rewrite H4 in H0; rewrite H1 in H0; simpl in H0; inversion H0;
-    rewrite <- H6 in H2; simpl in H2; try destruct H2.
-     * eapply (IHe1 F E s0); eauto.
-       intros; cset_tac. destruct (H x); eauto.
-     * eapply (IHe1 F E s); eauto.
-       intros; cset_tac; destruct (H x); eauto.
-     * pose proof (noguard_impl_eval  E e1).
-       destruct H5; eauto; isabsurd.
-       intros; cset_tac; destruct (H x); eauto.
-  + case_eq (undef e1); case_eq (undef e2); intros;
-    rewrite H4 in H0; rewrite H3 in H0; simpl in H0; inversion H0;
-    rewrite <- H6 in H2; simpl in H2; try destruct H2.
-    * eapply (IHe2 F E s); eauto.
-      intros; cset_tac. destruct (H x0); eauto.
-    * pose proof (noguard_impl_eval E e2).
-      destruct H5; eauto; isabsurd.
-      intros; cset_tac. destruct (H x0); eauto.
-    * eapply (IHe2 F E s); eauto.
-      intros; cset_tac. destruct (H x0); eauto.
-  + case_eq (undef e1); case_eq (undef e2); intros;
-    rewrite H4 in H0; rewrite H1 in H0; simpl in H0; inversion H0;
-    rewrite <- H6 in H2; simpl in H2; try destruct H2.
-     * eapply (IHe1 F E s0); eauto.
-       intros; cset_tac. destruct (H x); eauto.
-     * eapply (IHe1 F E s); eauto.
-       intros; cset_tac; destruct (H x); eauto.
-     * pose proof (noguard_impl_eval E e1).
-       destruct H5; eauto; isabsurd.
-       intros; cset_tac; destruct (H x); eauto.
-  +  case_eq (undef e1); case_eq (undef e2); intros;
-    rewrite H4 in H0; rewrite H3 in H0; simpl in H0; inversion H0;
-    rewrite <- H6 in H2; simpl in H2; try destruct H2.
-     * eapply (IHe2 F E s); eauto.
-       intros; cset_tac. destruct (H x0); eauto.
-     * pose proof (noguard_impl_eval E e2).
-       destruct H5; eauto; isabsurd.
-       intros; cset_tac. destruct (H x0); eauto.
-     * eapply (IHe2 F E s); eauto.
-       intros; cset_tac. destruct (H x0); eauto.
-  + case_eq (undef e1); case_eq (undef e2); intros;
-    rewrite H4 in H0; rewrite H1 in H0; simpl in H0; inversion H0;
-    rewrite <- H6 in H2; simpl in H2; try destruct H2.
-    * eapply (IHe1 F E s0); eauto.
-      intros; cset_tac. destruct (H x); eauto.
-    * eapply (IHe1 F E s); eauto.
-      intros; cset_tac; destruct (H x); eauto.
-    * pose proof (noguard_impl_eval E e1).
-      destruct H5; eauto; isabsurd.
-      intros; cset_tac; destruct (H x); eauto.
-  +  case_eq (undef e1); case_eq (undef e2); intros;
-    rewrite H4 in H0; rewrite H3 in H0; simpl in H0; inversion H0;
-    rewrite <- H6 in H2; simpl in H2; try destruct H2.
-     * eapply (IHe2 F E s); eauto.
-       intros; cset_tac. destruct (H x0); eauto.
-     * pose proof (noguard_impl_eval E e2).
-       destruct H5; eauto; isabsurd.
-       intros; cset_tac. destruct (H x0); eauto.
-     * eapply (IHe2 F E s); eauto.
-       intros; cset_tac. destruct (H x0); eauto.
-  + case_eq (undef e1); case_eq (undef e2); intros;
-    rewrite H1, H4 in H0; simpl in H0; inversion H0; clear H0;
-    rewrite <- H6 in H2; clear H6;
-    simpl in H2.
-    * destruct H2; destruct H2.  eapply (IHe1 F E s0); eauto.
-      intros; cset_tac. destruct (H x); eauto.
-    * destruct H2.  eapply (IHe1 F E s); eauto.
-      intros; cset_tac. destruct (H x); eauto.
-    * destruct H2. pose proof (noguard_impl_eval E e1); eauto.
-      destruct H5; eauto; isabsurd.
-      intros; cset_tac. destruct (H x); eauto.
-    * pose proof (noguard_impl_eval E e1).
-      destruct H0; eauto; isabsurd.
-      intros; cset_tac. destruct (H x); eauto.
-  +  case_eq (undef e1); case_eq (undef e2); intros;
-    rewrite H3, H4 in H0; simpl in H0; inversion H0; clear H0;
-    rewrite <- H6 in H2; clear H6;
-    simpl in H2; destruct H2; try destruct H2.
-     * eapply (IHe2 F E s); eauto.
-       intros; cset_tac. destruct (H x0); eauto.
-     * pose proof (noguard_impl_eval E e2).
-       destruct H5; eauto; isabsurd.
-       intros; cset_tac. destruct (H x0); eauto.
-     * eapply (IHe2 F E s); eauto.
-       intros; cset_tac. destruct (H x0); eauto.
-     * pose proof (noguard_impl_eval E e2).
-       destruct H0; eauto; isabsurd.
-       intros; cset_tac. destruct (H x0); eauto.
-  + case_eq (undef e1); case_eq (undef e2); intros;
-    rewrite H1, H3 in H0; simpl in H; inversion H0; clear H0;
-    rewrite <- H5 in H2; destruct H2; try destruct H2; clear H5.
-    * simpl in H1. destruct H1. simpl in EQ2. unfold bvDiv in EQ2.
-      apply H0.  case_eq(bvZero x0); intros.
-      Focus 2. rewrite H1 in EQ2. destruct (bvLessZero x); destruct (bvLessZero x0); isabsurd.
-      unfold evalSexp. rewrite EQ1. simpl.
-      change (val2bool (bvEq x0 (zext k (O::nil)))). clear H.  eapply zero_implies_eq; eauto.
-    * simpl in H1. destruct H1. simpl in EQ2. unfold bvDiv in EQ2.
-      apply H0.  case_eq(bvZero x0); intros.
-      Focus 2. rewrite H1 in EQ2. destruct (bvLessZero x); destruct (bvLessZero x0); isabsurd.
-      unfold evalSexp. rewrite EQ1. simpl.
-      change (val2bool (bvEq x0 (zext k (O::nil)))). clear H.  eapply zero_implies_eq; eauto.
-    * simpl in H1. destruct H1. simpl in EQ2. unfold bvDiv in EQ2.
-      apply H0.  case_eq(bvZero x0); intros.
-      Focus 2. rewrite H1 in EQ2. destruct (bvLessZero x); destruct (bvLessZero x0); isabsurd.
-      unfold evalSexp. rewrite EQ1. simpl.
-      change (val2bool (bvEq x0 (zext k (O::nil)))). clear H.  eapply zero_implies_eq; eauto.
-    * simpl in H1. destruct H1. simpl in EQ2. unfold bvDiv in EQ2.
-      case_eq(bvZero x0); intros.
-      Focus 2. rewrite H0 in EQ2. destruct (bvLessZero x); destruct (bvLessZero x0); isabsurd.
-      unfold evalSexp. rewrite EQ1. simpl.
-      change (val2bool (bvEq x0 (zext k (O::nil)))).  eapply zero_implies_eq; eauto.
-Qed.
-
-Lemma undefList_models:
-  forall F E el gl,
-    (forall x, x ∈ list_union (List.map Exp.freeVars el) -> exists v, E x = Some v)
-    -> undefLift el = Some gl
-    -> omap (exp_eval E) el = None
-    -> ~ models F E gl.
-
-Proof.
-  intros.
-  general induction el; simpl in *.
-  - case_eq (undef a); case_eq (undefLift el); intros;
-    rewrite H2, H3 in H0; simpl in H0; inversion H0; simpl; hnf; intros.
-    + destruct H4.
-      monad_inv (H1); isabsurd.
-      * pose proof (undef_models F E a s0).
-        eapply H1; eauto. setSubstUnion H.
-      * exploit (IHel F E s); eauto.
-        setSubstUnion H.
-    +  rewrite <- H5 in H4.
-      monad_inv H1; isabsurd.
-      * pose proof (undef_models F E a s).
-        eapply H1; eauto.
-        setSubstUnion H.
-      * pose proof (noguardlist_impl_eval E el).
-        destruct H6; eauto; isabsurd.
-        setSubstUnion H.
-    + monad_inv H1; isabsurd.
-      * pose proof (noguard_impl_eval E a).
-        destruct H1; eauto; isabsurd.
-        setSubstUnion H.
-      * exploit (IHel F E s); eauto; isabsurd.
-        setSubstUnion H.
-Qed.
-
-Lemma nostep_let:
-forall L E x e s,
-normal2 F.step (L, E, stmtExp x e s)
--> exp_eval E e = None.
-
-Proof.
-intros. case_eq (exp_eval E e); intros; eauto.
-exfalso; apply H. unfold reducible2.
-exists EvtTau. exists (L, E[x<-Some v],s). econstructor; eauto.
-Qed.
-
-Lemma nostep_if:
-forall L E e t f,
-normal2 F.step (L, E, stmtIf e t f)
--> exp_eval E e = None.
-
-Proof.
-intros. case_eq (exp_eval E e); intros; eauto.
-exfalso; eapply H; unfold reducible2.
-exists (EvtTau).
-case_eq (val2bool v); intros.
-- exists (L, E, t); econstructor; eauto.
-- exists (L, E, f); econstructor; eauto.
-Qed.
-
-Lemma noFun_Crash_tonil:
-forall L E s L' E' s',
-noFun s
--> Terminates (L, E, s) (L', E', s')
--> Terminates (nil, E, s) (nil, E', s').
-
-Proof.
-  intros L E s L' E' s' nf term.
-  general induction term.
-  - econstructor; eauto.
-  - econstructor; eauto.
-  - inversion nf;  subst;  invt F.step; try isabsurd.
-    + exploit (IHterm L' (E0[x<- Some v])  s'); eauto.
-      econstructor; eauto. instantiate (1:=EvtTau).
-      inversion H; econstructor; eauto.
-    + exploit (IHterm L' E' s'); eauto.
-      econstructor; eauto. instantiate (1:= EvtTau).
-      inversion H.
-      * econstructor; eauto.
-      * eapply F.stepIfF; eauto.
-    + exploit (IHterm L' E' s'); eauto.
-      econstructor; eauto. instantiate (1:=EvtTau).
-      inversion H.
-      * econstructor; eauto.
-      * eapply F.stepIfF; eauto.
-Qed.
-
-Lemma noFun_nil E s σ a:
-  noFun s
-  -> star2 F.step (nil, E,s) a σ
-  -> a = nil.
-
-Proof.
-  intros; general induction H0; invt noFun; eauto; isabsurd;
-  inv H; simpl; exploit IHstar2; try reflexivity; eauto.
-Qed.
-
-Lemma star2_noFun_Term:
-forall E s Es s',
-noFun s
--> Terminates (nil , E, s) (nil , Es, s')
--> star2 F.step  (nil, E, s) nil (nil, Es, s') /\
-   ((exists e, s' = stmtReturn e) \/ (exists f X, s' = stmtGoto f X)).
-
-Proof.
-  intros.
-  exploit terminates_impl_star2; eauto.
-Qed.
-
-Definition failed (σ:F.state)  := result (σ ) = None.
-
-Lemma crash_impl_err:
-  forall (E:onv val) s Es s' L L',
-    noFun s
-    -> Crash (L, E, s) (L', Es, s')
-    -> ( star2 F.step (L,E,s) nil (L', Es, s'))
-       /\ normal2 F.step (L', Es, s') /\ failed (L', Es, s').
-
-Proof.
-  intros E s Es s' L L' nf Crash.
-  general induction Crash.
-  - split; econstructor.
-    +  hnf. intros. destruct H0. destruct H0. inversion H0.
-       rewrite H in def; isabsurd.
-    + unfold failed; eauto.
-   - split; eauto;  econstructor.
-- destruct sigma'. destruct p. inversion nf; subst; try isabsurd.
-  + exploit (IHCrash o s1 Es s' l L') ; try reflexivity; eauto; subst.
-    * inversion H; eauto.
-    * destruct X; split; eauto.
-      change (star2 F.step (L0, E0, stmtExp x e s1) (filter_tau EvtTau nil) (L', Es, s')).
-      econstructor; eauto. destruct a; eauto; isabsurd.
-  + inversion H; exploit (IHCrash o s Es s' l L'); subst; eauto.
-    * destruct X; split; eauto.
-      change (star2 F.step (l, o, stmtIf e s t) (filter_tau EvtTau nil) (L', Es, s')).
-      econstructor; eauto.
-    * destruct X; split; eauto.
-      change (star2 F.step (l, o, stmtIf e s1 s) (filter_tau EvtTau nil) (L', Es, s')).
-      econstructor; eauto.
-Qed.
-
-Lemma star2_noFun_Crash:
-forall E s Es s',
-noFun s
--> Crash (nil, E, s) (nil, Es, s')
--> star2 F.step (nil, E, s) nil (nil, Es, s') /\
-   (normal2 F.step (nil, Es, s') /\ failed (nil, Es, s')).
-
-Proof.
-  intros.
-  exploit crash_impl_err; eauto.
-Qed.
-
-Lemma crash_impl_models:
-  forall L L' D s E Es s',
-    ssa s D
-    -> (forall x, x ∈ fst(getAnn D) -> exists v, E x = Some v)
-    -> noFun s
-    -> Crash (L, E, s) (L', Es, s')
-    -> models (fun _ => fun _ => true) Es (translateStmt s target).
-
-Proof.
-  intros. general induction H2; simpl.
-  - case_eq (undefLift Y); intros; simpl; intros; eauto.
-    + pose proof (undefList_models (fun _ => fun _ => true) E0 Y s).
-      eapply H6; eauto.
-      intros. eapply H1. inversion H0.
-      simpl. eauto.
-    + pose proof (noguardlist_impl_eval E0 Y).
-      destruct H5; eauto; isabsurd.
-      intros; eapply H1. inversion H0; simpl; eauto.
-  - inversion H4; subst.
-    + case_eq (undef e); simpl; intros.
-      * pose proof (nostep_let L0 E0 x e s H0).
-        pose proof (undef_models (fun _ => fun _ => true) E0 e s0).
-        assert (forall x, x ∈ Exp.freeVars e -> exists v, E0 x = Some v).
-        { intros; invt ssa. specialize (H3 x0). eapply H3.
-          simpl; cset_tac; eauto. }
-        { rewrite H6.  simpl.  intros. specialize (H8 H9 H6 H7 H10); isabsurd. }
-      * pose proof (noguard_impl_eval E0 e).
-        assert (forall x, x ∈ Exp.freeVars e -> exists v, E0 x = Some v).
-        { intros. inversion H2. specialize (H3 x0). subst. simpl in H3.
-          hnf in H13.  specialize (H13 x0 H8).  destruct (H3 H13).
-          exists x1; eauto. }
-        { specialize (H7 H8 H6). destruct H7.
-        assert (exists y σ, F.step (L0, E0, stmtExp x e s) y σ )
-            by (exists EvtTau; exists (L0, E0[x<-Some x0], s); econstructor; eauto ).
-          hnf in H0.  unfold reducible2 in H0. specialize (H0 H9); isabsurd. }
-    + case_eq (undef e); simpl; intros.
-      * pose proof (nostep_if L0 E0 e s t H0).
-        pose proof (undef_models (fun _ => fun _ => true) E0 e s0).
-        assert (forall x, x ∈ Exp.freeVars e -> exists v, E0 x = Some v).
-        { intros; invt ssa. eapply (H3 x). simpl; cset_tac; eauto. }
-        { rewrite H7; simpl; intros. specialize (H9 H10 H7 H8 H11); isabsurd. }
-      * pose proof (noguard_impl_eval E0 e).
-        assert (forall x, x ∈ Exp.freeVars e -> exists v, E0 x = Some v).
-        { intros; invt ssa. specialize (H3 x); subst; simpl in *. cset_tac.
-          hnf in H13. destruct (H3 (H13 x H9)).
-          exists x0. rewrite H10; eauto. }
-        { specialize (H8 H9 H7).
-        assert (exists y σ, F.step (L0, E0 , stmtIf e s t) y σ).
-        { exists EvtTau. destruct H8. case_eq (val2bool x); intros.
-          - exists (L0, E0, s). econstructor; eauto.
-          - exists (L0, E0, t). econstructor; eauto. }
-        { specialize (H0 H10); isabsurd. } }
-    + isabsurd.
-    +  case_eq (undef e); simpl; intros.
-       * pose proof (undef_models (fun _ => fun _ => true) E0 e s).
-         assert (forall x, x ∈ Exp.freeVars e -> exists v, E0 x = Some v).
-        { intros; inversion H2; cset_tac.  simpl in H3. specialize (H3 x).
-        destruct H1; eauto. }
-       { rewrite H5; simpl. specialize (H6 H7 H5 H1); isabsurd. }
-       * pose proof (noguard_impl_eval E0 e).
-         assert (forall x, x ∈ Exp.freeVars e -> exists v, E0 x = Some v).
-         { intros. inversion H2. simpl in H3. specialize (H3 x).
-           hnf in H9. cset_tac. destruct H3; eauto. }
-         { simpl in H3. specialize (H6 H7). specialize (H6 H5).
-           destruct H6. rewrite H5; simpl; intros. simpl in H1.
-           rewrite H6 in H1; isabsurd. }
-  - destruct sigma' as  [[L E'] sc].
-    case_eq s0; intros; subst; simpl in*; invt ssa; invt noFun; invt F.step; subst.
-    + exploit (IHCrash L L' an sc (E0 [x<-Some v]) Es s'); eauto; intros.
-      * rewrite H12 in H5.  simpl in H5.  cset_tac.  destruct H5.
-        { inversion H; subst.  simpl in H3; specialize (H3 x0 H5).
-          destruct H3. exists x1. unfold update.
-          decide (x === x0); eauto; isabsurd. }
-        { rewrite H5. unfold update.
-          decide (x === x); isabsurd.
-          exists v; eauto. }
-      * case_eq (undef e); intros.
-        { simpl; split; eauto. unfold evalSexp.
-          assert ( exp_eval Es e = Some v /\ exp_eval Es (Var x) = Some v).
-          - split.
-            + eapply (exp_eval_agree (E:=E0)); eauto.
-            hnf. intros.  hnf in H9. specialize (H9 x0 H10).
-            pose proof (crash_ssa_eval_agree L L' (stmtExp x e sc) (ann1 (D0, D') an) s' E0 Es).
-            eapply H13; eauto; econstructor; eauto.
-            +  eapply (exp_eval_agree (E:= E0[x<-Some v])).
-              * hnf. intros; simpl in H10.
-                eapply (crash_ssa_eval_agree L L' sc an s' (E0[x<-Some v]) Es); eauto.
-                rewrite H12; simpl. cset_tac. right. rewrite H10; eauto.
-              * simpl. unfold update. decide (x === x); eauto; isabsurd.
-          - destruct H10.  rewrite H10, H13.  eapply bvEq_equiv_eq; eauto. }
-        { simpl; split; eauto. unfold evalSexp. inversion H.
-          assert ( exp_eval Es e = Some v).
-          - eapply (exp_eval_agree (E:= E0)); eauto.
-            hnf. intros.  hnf in H9. specialize (H9 x1 H7).
-            pose proof (crash_ssa_eval_agree L L' (stmtExp x e sc) (ann1 (D0, D') an) s' E0 Es).
-            eapply H18; eauto; econstructor;  eauto.
-          - assert (exp_eval Es (Var x) =Some v).
-            + eapply (exp_eval_agree (E:= E0[x<-Some v])).
-              * hnf. intros. simpl in H18. cset_tac.
-                eapply (crash_ssa_eval_agree L L' sc an s' (E0[x<-Some v]) Es); eauto.
-                rewrite H12; simpl. cset_tac. right. rewrite H18; eauto.
-              * simpl. unfold update. decide (x === x).
-                { reflexivity. }
-                { isabsurd. }
-            + rewrite H18, H7. eapply bvEq_equiv_eq.
-              reflexivity. }
-    +  exploit (IHCrash L L' ans sc E' Es s'); eauto.
-       * intros. rewrite H14 in H5. simpl in *; eauto.
-       * case_eq (undef e); intros; simpl; unfold evalSexp.
-         { assert (exp_eval Es e = Some v).
-           - eapply (exp_eval_agree (E:= E')); eauto.
-             hnf; intros.  hnf in H8.  specialize (H8 x H6).
-             pose proof (crash_ssa_eval_agree L L' (stmtIf e sc t) (ann2 (D0, D') ans ant) s'  E' Es).
-             eapply H13; eauto; econstructor; eauto.
-           - rewrite H6.  rewrite condTrue.  intros; subst; eauto. }
-         { assert (exp_eval Es e = Some v).
-           - eapply (exp_eval_agree (E:= E')); eauto.
-             hnf; intros.  hnf in H8.  specialize (H8 x H6).
-             pose proof (crash_ssa_eval_agree L L' (stmtIf e sc t) (ann2 (D0, D') ans ant) s'  E' Es).
-             eapply H13; eauto; econstructor; eauto.
-           - rewrite H6.  rewrite condTrue.  intros; subst; eauto. }
-    + exploit (IHCrash L L' ant sc E' Es s'); eauto.
-      * intros. rewrite H15 in H5; simpl in *; eauto.
-      *  case_eq (undef e); intros; simpl; unfold evalSexp.
-         {  assert (exp_eval Es e = Some v).
-            - eapply (exp_eval_agree (E:= E')); eauto.
-              hnf; intros.  hnf in H8.  specialize (H8 x H6).
-              pose proof (crash_ssa_eval_agree L L' (stmtIf e s sc) (ann2 (D0, D') ans ant) s'  E' Es).
-              eapply H13; eauto; econstructor; eauto.
-            - rewrite H6.  rewrite condFalse. intros; subst; eauto. }
-         { assert (exp_eval Es e = Some v).
-           - eapply (exp_eval_agree (E:= E')); eauto.
-             hnf; intros.  hnf in H8.  specialize (H8 x H6).
-              pose proof (crash_ssa_eval_agree L L' (stmtIf e s sc) (ann2 (D0, D') ans ant) s'  E' Es).
-              eapply H13; eauto; econstructor; eauto.
-           - rewrite H6.  rewrite condFalse.  intros; subst; eauto. }
-    + isabsurd.
-Qed.
 
 Lemma noFun_impl_term_crash :
 forall E s,
@@ -1253,6 +626,13 @@ Proof.
                   try isabsurd; econstructor; eauto.
 Qed.
 
+Lemma combineenv_agree D E E':
+  agree_on eq D (combineEnv D E E') E.
+
+Proof.
+  hnf; intros. unfold combineEnv. destruct if; eauto; isabsurd.
+Qed.
+
 Lemma exp_combineenv_eql:
 forall e D Es Et v,
 Exp.freeVars e ⊆ D
@@ -1261,15 +641,12 @@ Exp.freeVars e ⊆ D
 Proof.
   intros. split; intros.
   - eapply (exp_eval_agree (E:=(combineEnv D Es Et))); eauto.
-  hnf. cset_tac. unfold combineEnv. hnf in H. specialize (H x H1).
-  decide (x ∈ D).
-    + reflexivity.
-    + exfalso. eapply n; assumption.
+    eapply (agree_on_incl (bv:= Exp.freeVars e) (lv:= D));
+      cset_tac; eauto.
+    eapply combineenv_agree.
   - eapply (exp_eval_agree (E:=Es)); eauto.
-    hnf; cset_tac; unfold combineEnv; hnf in H. specialize (H x H1).
-    decide (x ∈ D).
-    + reflexivity.
-    + exfalso; eapply n; assumption.
+    eapply (agree_on_incl (bv:=Exp.freeVars e) (lv:=D)); eauto.
+    symmetry. eapply combineenv_agree.
 Qed.
 
   Lemma explist_combineenv_eql:
@@ -1279,26 +656,55 @@ list_union (List.map Exp.freeVars el) ⊆ D
 
 Proof.
   intros; split; intros.
-  - general induction el.
-    + simpl. reflexivity.
+  - general induction el; eauto.
     + simpl. simpl in H. hnf in H.
       pose proof (exp_combineenv_eql a D Es Et (exp_eval (combineEnv D Es Et) a)); eauto.
-      destruct H0.
-      * hnf. intros. eapply H. unfold list_union; simpl.
-        eapply list_union_start_swap. cset_tac. left; right; eauto.
-      * rewrite H0; eauto.  erewrite IHel ; eauto.
-        hnf. intros. eapply H. unfold list_union. simpl. eapply list_union_start_swap.
-        cset_tac. right; assumption.
-  - general induction el.
-    + simpl; reflexivity.
+      destruct H0; hnf; intros; try setSubstUnion H.
+      * rewrite H0; eauto. erewrite IHel ; eauto.
+        hnf; intros. setSubstUnion H.
+  - general induction el; eauto.
     + simpl; simpl in H; hnf in H;  unfold evalSexp.
       pose proof (exp_combineenv_eql a D Es Et (exp_eval (combineEnv D Es Et) a)); eauto.
-      destruct H0.
-      * hnf; intros; eapply H; unfold list_union; simpl.
-        eapply list_union_start_swap; cset_tac. left; right; eauto.
+      destruct H0; hnf; intros; try setSubstUnion H.
       * rewrite H0; eauto. erewrite IHel; eauto.
-        hnf. intros. eapply H. unfold list_union. simpl. eapply list_union_start_swap.
-        cset_tac. right; assumption.
+        hnf; intros; setSubstUnion H.
+Qed.
+
+Lemma models_agree F E E' s:
+  agree_on eq (freeVars s) E E'
+  -> (models F E s <-> models F E' s).
+
+Proof.
+intros agree; general  induction s; simpl in *; try reflexivity.
+- rewrite (IHs1 F E E'), (IHs2 F E E'); try reflexivity; setSubst2 agree.
+- rewrite (IHs1 F E E'), (IHs2 F E E'); try reflexivity; setSubst2 agree.
+- rewrite (IHs F E E'); try reflexivity; setSubst2 agree.
+- assert (agree_on eq (Exp.freeVars e) E E') by setSubst2 agree.
+  assert (exp_eval E e = exp_eval E' e)
+  by( eapply exp_eval_agree; symmetry; eauto).
+  case_eq (exp_eval E e); intros; unfold evalSexp.
+  +  rewrite <- H0. rewrite H1. case_eq(val2bool v); intros.
+     * rewrite (IHs1 F E E'); try reflexivity; setSubst2 agree.
+     * rewrite (IHs2 F E E'); try reflexivity; setSubst2 agree.
+  + rewrite <- H0; rewrite H1; simpl.
+    rewrite (IHs2 F E E'); try reflexivity; setSubst2 agree.
+- rewrite (IHs1 F E E'), (IHs2 F E E'); try reflexivity; setSubst2 agree.
+-  assert (exp_eval E e = exp_eval E' e)
+    by ( eapply exp_eval_agree; symmetry; eauto; setSubst2 agree).
+  assert (exp_eval E e0 = exp_eval E' e0)
+    by (eapply exp_eval_agree; symmetry; eauto; setSubst2 agree).
+  unfold evalSexp; rewrite <- H; rewrite <- H0.
+  unfold val2bool.
+  case_eq (exp_eval E e); case_eq (exp_eval E e0); intros;
+  rewrite bvEq_equiv_eq; reflexivity.
+- unfold evalSpred. destruct p.  unfold evalList.
+  assert (omap (exp_eval E) a = omap (exp_eval E')  a).
+  + eapply omap_exp_eval_agree; symmetry; eauto.
+  + rewrite <- H. destruct (omap (exp_eval E) a); reflexivity.
+- unfold evalSexp.
+  assert (exp_eval E e = exp_eval E' e)
+    by (eapply  exp_eval_agree; symmetry; eauto; setSubst2 agree).
+  rewrite <- H. case_eq (exp_eval E e); intros; reflexivity.
 Qed.
 
 Lemma combineenv_eql:
@@ -1307,6 +713,8 @@ forall F s D Es Et,
 ->(  models F Es s  <-> models F (combineEnv D Es Et) s).
 
 Proof.
+  intros. eapply models_agree. eapply (agree_on_incl (lv:=D)); eauto; symmetry;
+eapply combineenv_agree.
 intros.  general induction s; simpl; try reflexivity.
 - rewrite (IHs1 F D Es Et). rewrite (IHs2 F D Es Et).
   + reflexivity.
