TransVal/crashProps.v
@@ -1,0 +1,431 @@
+Require Import List Arith.
+Require Import IL Annotation AutoIndTac Bisim Exp MoreExp Coherence Fresh Util.
+Require Import SetOperations Sim Var.
+Require Import sexp smt nofun noGoto Terminates bitvec Crash freeVars.
+Require Import tvalTactics TUtil Guards.
+
+Definition failed (σ:F.state)  := result (σ ) = None.
+
+Lemma crash_ssa_eval_agree L L' s D s' (E:onv val) (E':onv val)
+: ssa s D
+  ->noFun s
+  -> Crash (L, E, s) (L', E', s')
+  -> agree_on eq (fst (getAnn (D))) E E'.
+
+Proof.
+  intros.
+  general induction H1; invt ssa; try invt F.step; try invt noFun; simpl;
+  try reflexivity; isabsurd.
+  - exploit IHCrash; [ | | reflexivity | reflexivity |]; eauto.
+    rewrite H7 in X; simpl in *; cset_tac; intuition.
+    hnf; hnf in X; intros.
+    unfold update in X; specialize (X x0).
+    assert (x0 ∈ D0 ++ {x; {}}) by (cset_tac; left; assumption).
+    specialize (X H10); decide (x === x0); eauto.
+    + rewrite <- e0 in H8; exfalso; eapply H4; assumption.
+  - exploit IHCrash; [ | | reflexivity | reflexivity |]; eauto.
+    rewrite H9 in X; eauto.
+  - exploit IHCrash; [ | | reflexivity | reflexivity |]; eauto.
+    rewrite H10 in X; eauto.
+Qed.
+
+Lemma undef_models:
+forall F E e g,
+(forall x, x ∈ Exp.freeVars e -> exists v, E x = Some v)
+-> undef e =Some g
+-> exp_eval E e = None
+-> ~ models F E g.
+
+Proof.
+intros;  hnf;  intros.
+general induction e; simpl in *; try isabsurd.
+- monad_inv H1.
+  + specialize (IHe F E g H H0 H3 H2); eauto.
+  + destruct u; isabsurd.
+- destructBin b; monad_inv H1; try isabsurd.
+  + case_eq (undef e1); case_eq (undef e2); intros;
+    rewrite H4 in H0; rewrite H1 in H0; simpl in H0; inversion H0;
+    rewrite <- H6 in H2; simpl in H2; try destruct H2.
+    * eapply (IHe1 F E s0); eauto.
+      intros. cset_tac. specialize (H x). destruct H; eauto.
+    * eapply (IHe1 F E s); eauto.
+      intros; cset_tac; specialize (H x); destruct H; eauto.
+    * pose proof (noguard_impl_eval  E e1).
+      destruct H5; isabsurd; eauto.
+      intros; cset_tac; destruct (H x); eauto.
+  + case_eq (undef e1); case_eq (undef e2); intros;
+    rewrite H4 in H0; rewrite H3 in H0; simpl in H0; inversion H0;
+    rewrite <- H6 in H2; simpl in H2; try destruct H2.
+    * eapply (IHe2 F E s); eauto.
+      intros; cset_tac. destruct (H x0); eauto.
+    * pose proof (noguard_impl_eval E e2).
+      destruct H5; isabsurd; eauto.
+      intros; cset_tac. destruct (H x0); eauto.
+    * eapply (IHe2 F E s); eauto.
+      intros; cset_tac. destruct (H x0); eauto.
+  +  case_eq (undef e1); case_eq (undef e2); intros;
+    rewrite H4 in H0; rewrite H1 in H0; simpl in H0; inversion H0;
+    rewrite <- H6 in H2; simpl in H2; try destruct H2.
+     * eapply (IHe1 F E s0); eauto.
+       intros; cset_tac. destruct (H x); eauto.
+     * eapply (IHe1 F E s); eauto.
+       intros; cset_tac; destruct (H x); eauto.
+     * pose proof (noguard_impl_eval E e1).
+       destruct H5; eauto; isabsurd.
+       intros; cset_tac; destruct (H x); eauto.
+  + case_eq (undef e1); case_eq (undef e2); intros;
+    rewrite H4 in H0; rewrite H3 in H0; simpl in H0; inversion H0;
+    rewrite <- H6 in H2; simpl in H2; try destruct H2.
+    * eapply (IHe2 F E s); eauto.
+      intros; cset_tac. destruct (H x0); eauto.
+    * pose proof (noguard_impl_eval E e2).
+      destruct H5; eauto; isabsurd.
+      intros; cset_tac. destruct (H x0); eauto.
+    * eapply (IHe2 F E s); eauto.
+      intros; cset_tac. destruct (H x0); eauto.
+  + case_eq (undef e1); case_eq (undef e2); intros;
+    rewrite H4 in H0; rewrite H1 in H0; simpl in H0; inversion H0;
+    rewrite <- H6 in H2; simpl in H2; try destruct H2.
+     * eapply (IHe1 F E s0); eauto.
+       intros; cset_tac. destruct (H x); eauto.
+     * eapply (IHe1 F E s); eauto.
+       intros; cset_tac; destruct (H x); eauto.
+     * pose proof (noguard_impl_eval  E e1).
+       destruct H5; eauto; isabsurd.
+       intros; cset_tac; destruct (H x); eauto.
+  + case_eq (undef e1); case_eq (undef e2); intros;
+    rewrite H4 in H0; rewrite H3 in H0; simpl in H0; inversion H0;
+    rewrite <- H6 in H2; simpl in H2; try destruct H2.
+    * eapply (IHe2 F E s); eauto.
+      intros; cset_tac. destruct (H x0); eauto.
+    * pose proof (noguard_impl_eval E e2).
+      destruct H5; eauto; isabsurd.
+      intros; cset_tac. destruct (H x0); eauto.
+    * eapply (IHe2 F E s); eauto.
+      intros; cset_tac. destruct (H x0); eauto.
+  + case_eq (undef e1); case_eq (undef e2); intros;
+    rewrite H4 in H0; rewrite H1 in H0; simpl in H0; inversion H0;
+    rewrite <- H6 in H2; simpl in H2; try destruct H2.
+     * eapply (IHe1 F E s0); eauto.
+       intros; cset_tac. destruct (H x); eauto.
+     * eapply (IHe1 F E s); eauto.
+       intros; cset_tac; destruct (H x); eauto.
+     * pose proof (noguard_impl_eval E e1).
+       destruct H5; eauto; isabsurd.
+       intros; cset_tac; destruct (H x); eauto.
+  +  case_eq (undef e1); case_eq (undef e2); intros;
+    rewrite H4 in H0; rewrite H3 in H0; simpl in H0; inversion H0;
+    rewrite <- H6 in H2; simpl in H2; try destruct H2.
+     * eapply (IHe2 F E s); eauto.
+       intros; cset_tac. destruct (H x0); eauto.
+     * pose proof (noguard_impl_eval E e2).
+       destruct H5; eauto; isabsurd.
+       intros; cset_tac. destruct (H x0); eauto.
+     * eapply (IHe2 F E s); eauto.
+       intros; cset_tac. destruct (H x0); eauto.
+  + case_eq (undef e1); case_eq (undef e2); intros;
+    rewrite H4 in H0; rewrite H1 in H0; simpl in H0; inversion H0;
+    rewrite <- H6 in H2; simpl in H2; try destruct H2.
+    * eapply (IHe1 F E s0); eauto.
+      intros; cset_tac. destruct (H x); eauto.
+    * eapply (IHe1 F E s); eauto.
+      intros; cset_tac; destruct (H x); eauto.
+    * pose proof (noguard_impl_eval E e1).
+      destruct H5; eauto; isabsurd.
+      intros; cset_tac; destruct (H x); eauto.
+  +  case_eq (undef e1); case_eq (undef e2); intros;
+    rewrite H4 in H0; rewrite H3 in H0; simpl in H0; inversion H0;
+    rewrite <- H6 in H2; simpl in H2; try destruct H2.
+     * eapply (IHe2 F E s); eauto.
+       intros; cset_tac. destruct (H x0); eauto.
+     * pose proof (noguard_impl_eval E e2).
+       destruct H5; eauto; isabsurd.
+       intros; cset_tac. destruct (H x0); eauto.
+     * eapply (IHe2 F E s); eauto.
+       intros; cset_tac. destruct (H x0); eauto.
+  + case_eq (undef e1); case_eq (undef e2); intros;
+    rewrite H1, H4 in H0; simpl in H0; inversion H0; clear H0;
+    rewrite <- H6 in H2; clear H6;
+    simpl in H2.
+    * destruct H2; destruct H2.  eapply (IHe1 F E s0); eauto.
+      intros; cset_tac. destruct (H x); eauto.
+    * destruct H2.  eapply (IHe1 F E s); eauto.
+      intros; cset_tac. destruct (H x); eauto.
+    * destruct H2. pose proof (noguard_impl_eval E e1); eauto.
+      destruct H5; eauto; isabsurd.
+      intros; cset_tac. destruct (H x); eauto.
+    * pose proof (noguard_impl_eval E e1).
+      destruct H0; eauto; isabsurd.
+      intros; cset_tac. destruct (H x); eauto.
+  +  case_eq (undef e1); case_eq (undef e2); intros;
+    rewrite H3, H4 in H0; simpl in H0; inversion H0; clear H0;
+    rewrite <- H6 in H2; clear H6;
+    simpl in H2; destruct H2; try destruct H2.
+     * eapply (IHe2 F E s); eauto.
+       intros; cset_tac. destruct (H x0); eauto.
+     * pose proof (noguard_impl_eval E e2).
+       destruct H5; eauto; isabsurd.
+       intros; cset_tac. destruct (H x0); eauto.
+     * eapply (IHe2 F E s); eauto.
+       intros; cset_tac. destruct (H x0); eauto.
+     * pose proof (noguard_impl_eval E e2).
+       destruct H0; eauto; isabsurd.
+       intros; cset_tac. destruct (H x0); eauto.
+  + case_eq (undef e1); case_eq (undef e2); intros;
+    rewrite H1, H3 in H0; simpl in H; inversion H0; clear H0;
+    rewrite <- H5 in H2; destruct H2; try destruct H2; clear H5.
+    * simpl in H1. destruct H1. simpl in EQ2. unfold bvDiv in EQ2.
+      apply H0.  case_eq(bvZero x0); intros.
+      Focus 2. rewrite H1 in EQ2. destruct (bvLessZero x); destruct (bvLessZero x0); isabsurd.
+      unfold evalSexp. rewrite EQ1. simpl.
+      change (val2bool (bvEq x0 (zext k (O::nil)))). clear H.  eapply zero_implies_eq; eauto.
+    * simpl in H1. destruct H1. simpl in EQ2. unfold bvDiv in EQ2.
+      apply H0.  case_eq(bvZero x0); intros.
+      Focus 2. rewrite H1 in EQ2. destruct (bvLessZero x); destruct (bvLessZero x0); isabsurd.
+      unfold evalSexp. rewrite EQ1. simpl.
+      change (val2bool (bvEq x0 (zext k (O::nil)))). clear H.  eapply zero_implies_eq; eauto.
+    * simpl in H1. destruct H1. simpl in EQ2. unfold bvDiv in EQ2.
+      apply H0.  case_eq(bvZero x0); intros.
+      Focus 2. rewrite H1 in EQ2. destruct (bvLessZero x); destruct (bvLessZero x0); isabsurd.
+      unfold evalSexp. rewrite EQ1. simpl.
+      change (val2bool (bvEq x0 (zext k (O::nil)))). clear H.  eapply zero_implies_eq; eauto.
+    * simpl in H1. destruct H1. simpl in EQ2. unfold bvDiv in EQ2.
+      case_eq(bvZero x0); intros.
+      Focus 2. rewrite H0 in EQ2. destruct (bvLessZero x); destruct (bvLessZero x0); isabsurd.
+      unfold evalSexp. rewrite EQ1. simpl.
+      change (val2bool (bvEq x0 (zext k (O::nil)))).  eapply zero_implies_eq; eauto.
+Qed.
+
+Lemma undefList_models:
+  forall F E el gl,
+    (forall x, x ∈ list_union (List.map Exp.freeVars el) -> exists v, E x = Some v)
+    -> undefLift el = Some gl
+    -> omap (exp_eval E) el = None
+    -> ~ models F E gl.
+
+Proof.
+  intros.
+  general induction el; simpl in *.
+  - case_eq (undef a); case_eq (undefLift el); intros;
+    rewrite H2, H3 in H0; simpl in H0; inversion H0; simpl; hnf; intros.
+    + destruct H4.
+      monad_inv (H1); isabsurd.
+      * pose proof (undef_models F E a s0).
+        eapply H1; eauto. setSubstUnion H.
+      * exploit (IHel F E s); eauto.
+        setSubstUnion H.
+    +  rewrite <- H5 in H4.
+      monad_inv H1; isabsurd.
+      * pose proof (undef_models F E a s).
+        eapply H1; eauto.
+        setSubstUnion H.
+      * pose proof (noguardlist_impl_eval E el).
+        destruct H6; eauto; isabsurd.
+        setSubstUnion H.
+    + monad_inv H1; isabsurd.
+      * pose proof (noguard_impl_eval E a).
+        destruct H1; eauto; isabsurd.
+        setSubstUnion H.
+      * exploit (IHel F E s); eauto; isabsurd.
+        setSubstUnion H.
+Qed.
+
+Lemma crash_impl_err:
+  forall (E:onv val) s Es s' L L',
+    noFun s
+    -> Crash (L, E, s) (L', Es, s')
+    -> ( star2 F.step (L,E,s) nil (L', Es, s'))
+       /\ normal2 F.step (L', Es, s') /\ failed (L', Es, s').
+
+Proof.
+  intros E s Es s' L L' nf Crash.
+  general induction Crash.
+  - split; econstructor.
+    +  hnf. intros. destruct H0. destruct H0. inversion H0.
+       rewrite H in def; isabsurd.
+    + unfold failed; eauto.
+   - split; eauto;  econstructor.
+- destruct sigma'. destruct p. inversion nf; subst; try isabsurd.
+  + exploit (IHCrash o s1 Es s' l L') ; try reflexivity; eauto; subst.
+    * inversion H; eauto.
+    * destruct X; split; eauto.
+      change (star2 F.step (L0, E0, stmtExp x e s1) (filter_tau EvtTau nil) (L', Es, s')).
+      econstructor; eauto. destruct a; eauto; isabsurd.
+  + inversion H; exploit (IHCrash o s Es s' l L'); subst; eauto.
+    * destruct X; split; eauto.
+      change (star2 F.step (l, o, stmtIf e s t) (filter_tau EvtTau nil) (L', Es, s')).
+      econstructor; eauto.
+    * destruct X; split; eauto.
+      change (star2 F.step (l, o, stmtIf e s1 s) (filter_tau EvtTau nil) (L', Es, s')).
+      econstructor; eauto.
+Qed.
+
+Lemma nostep_let:
+forall L E x e s,
+normal2 F.step (L, E, stmtExp x e s)
+-> exp_eval E e = None.
+
+Proof.
+intros. case_eq (exp_eval E e); intros; eauto.
+exfalso; apply H. unfold reducible2.
+exists EvtTau. exists (L, E[x<-Some v],s). econstructor; eauto.
+Qed.
+
+Lemma nostep_if:
+forall L E e t f,
+normal2 F.step (L, E, stmtIf e t f)
+-> exp_eval E e = None.
+
+Proof.
+intros. case_eq (exp_eval E e); intros; eauto.
+exfalso; eapply H; unfold reducible2.
+exists (EvtTau).
+case_eq (val2bool v); intros.
+- exists (L, E, t); econstructor; eauto.
+- exists (L, E, f); econstructor; eauto.
+Qed.
+
+Lemma crash_impl_models:
+  forall L L' D s E Es s',
+    ssa s D
+    -> (forall x, x ∈ fst(getAnn D) -> exists v, E x = Some v)
+    -> noFun s
+    -> Crash (L, E, s) (L', Es, s')
+    -> models (fun _ => fun _ => true) Es (translateStmt s target).
+
+Proof.
+  intros. general induction H2; simpl.
+  - case_eq (undefLift Y); intros; simpl; intros; eauto.
+    + pose proof (undefList_models (fun _ => fun _ => true) E0 Y s).
+      eapply H6; eauto.
+      intros. eapply H1. inversion H0.
+      simpl. eauto.
+    + pose proof (noguardlist_impl_eval E0 Y).
+      destruct H5; eauto; isabsurd.
+      intros; eapply H1. inversion H0; simpl; eauto.
+  - inversion H4; subst.
+    + case_eq (undef e); simpl; intros.
+      * pose proof (nostep_let L0 E0 x e s H0).
+        pose proof (undef_models (fun _ => fun _ => true) E0 e s0).
+        assert (forall x, x ∈ Exp.freeVars e -> exists v, E0 x = Some v).
+        { intros; invt ssa. specialize (H3 x0). eapply H3.
+          simpl; cset_tac; eauto. }
+        { rewrite H6.  simpl.  intros. specialize (H8 H9 H6 H7 H10); isabsurd. }
+      * pose proof (noguard_impl_eval E0 e).
+        assert (forall x, x ∈ Exp.freeVars e -> exists v, E0 x = Some v).
+        { intros. inversion H2. specialize (H3 x0). subst. simpl in H3.
+          hnf in H13.  specialize (H13 x0 H8).  destruct (H3 H13).
+          exists x1; eauto. }
+        { specialize (H7 H8 H6). destruct H7.
+        assert (exists y σ, F.step (L0, E0, stmtExp x e s) y σ )
+            by (exists EvtTau; exists (L0, E0[x<-Some x0], s); econstructor; eauto ).
+          hnf in H0.  unfold reducible2 in H0. specialize (H0 H9); isabsurd. }
+    + case_eq (undef e); simpl; intros.
+      * pose proof (nostep_if L0 E0 e s t H0).
+        pose proof (undef_models (fun _ => fun _ => true) E0 e s0).
+        assert (forall x, x ∈ Exp.freeVars e -> exists v, E0 x = Some v).
+        { intros; invt ssa. eapply (H3 x). simpl; cset_tac; eauto. }
+        { rewrite H7; simpl; intros. specialize (H9 H10 H7 H8 H11); isabsurd. }
+      * pose proof (noguard_impl_eval E0 e).
+        assert (forall x, x ∈ Exp.freeVars e -> exists v, E0 x = Some v).
+        { intros; invt ssa. specialize (H3 x); subst; simpl in *. cset_tac.
+          hnf in H13. destruct (H3 (H13 x H9)).
+          exists x0. rewrite H10; eauto. }
+        { specialize (H8 H9 H7).
+        assert (exists y σ, F.step (L0, E0 , stmtIf e s t) y σ).
+        { exists EvtTau. destruct H8. case_eq (val2bool x); intros.
+          - exists (L0, E0, s). econstructor; eauto.
+          - exists (L0, E0, t). econstructor; eauto. }
+        { specialize (H0 H10); isabsurd. } }
+    + isabsurd.
+    +  case_eq (undef e); simpl; intros.
+       * pose proof (undef_models (fun _ => fun _ => true) E0 e s).
+         assert (forall x, x ∈ Exp.freeVars e -> exists v, E0 x = Some v).
+        { intros; inversion H2; cset_tac.  simpl in H3. specialize (H3 x).
+        destruct H1; eauto. }
+       { rewrite H5; simpl. specialize (H6 H7 H5 H1); isabsurd. }
+       * pose proof (noguard_impl_eval E0 e).
+         assert (forall x, x ∈ Exp.freeVars e -> exists v, E0 x = Some v).
+         { intros. inversion H2. simpl in H3. specialize (H3 x).
+           hnf in H9. cset_tac. destruct H3; eauto. }
+         { simpl in H3. specialize (H6 H7). specialize (H6 H5).
+           destruct H6. rewrite H5; simpl; intros. simpl in H1.
+           rewrite H6 in H1; isabsurd. }
+  - destruct sigma' as  [[L E'] sc].
+    case_eq s0; intros; subst; simpl in*; invt ssa; invt noFun; invt F.step; subst.
+    + exploit (IHCrash L L' an sc (E0 [x<-Some v]) Es s'); eauto; intros.
+      * rewrite H12 in H5.  simpl in H5.  cset_tac.  destruct H5.
+        { inversion H; subst.  simpl in H3; specialize (H3 x0 H5).
+          destruct H3. exists x1. unfold update.
+          decide (x === x0); eauto; isabsurd. }
+        { rewrite H5. unfold update.
+          decide (x === x); isabsurd.
+          exists v; eauto. }
+      * case_eq (undef e); intros.
+        { simpl; split; eauto. unfold evalSexp.
+          assert ( exp_eval Es e = Some v /\ exp_eval Es (Var x) = Some v).
+          - split.
+            + eapply (exp_eval_agree (E:=E0)); eauto.
+            hnf. intros.  hnf in H9. specialize (H9 x0 H10).
+            pose proof (crash_ssa_eval_agree L L' (stmtExp x e sc) (ann1 (D0, D') an) s' E0 Es).
+            eapply H13; eauto; econstructor; eauto.
+            +  eapply (exp_eval_agree (E:= E0[x<-Some v])).
+              * hnf. intros; simpl in H10.
+                eapply (crash_ssa_eval_agree L L' sc an s' (E0[x<-Some v]) Es); eauto.
+                rewrite H12; simpl. cset_tac. right. rewrite H10; eauto.
+              * simpl. unfold update. decide (x === x); eauto; isabsurd.
+          - destruct H10.  rewrite H10, H13.  eapply bvEq_equiv_eq; eauto. }
+        { simpl; split; eauto. unfold evalSexp. inversion H.
+          assert ( exp_eval Es e = Some v).
+          - eapply (exp_eval_agree (E:= E0)); eauto.
+            hnf. intros.  hnf in H9. specialize (H9 x1 H7).
+            pose proof (crash_ssa_eval_agree L L' (stmtExp x e sc) (ann1 (D0, D') an) s' E0 Es).
+            eapply H18; eauto; econstructor;  eauto.
+          - assert (exp_eval Es (Var x) =Some v).
+            + eapply (exp_eval_agree (E:= E0[x<-Some v])).
+              * hnf. intros. simpl in H18. cset_tac.
+                eapply (crash_ssa_eval_agree L L' sc an s' (E0[x<-Some v]) Es); eauto.
+                rewrite H12; simpl. cset_tac. right. rewrite H18; eauto.
+              * simpl. unfold update. decide (x === x).
+                { reflexivity. }
+                { isabsurd. }
+            + rewrite H18, H7. eapply bvEq_equiv_eq.
+              reflexivity. }
+    +  exploit (IHCrash L L' ans sc E' Es s'); eauto.
+       * intros. rewrite H14 in H5. simpl in *; eauto.
+       * case_eq (undef e); intros; simpl; unfold evalSexp.
+         { assert (exp_eval Es e = Some v).
+           - eapply (exp_eval_agree (E:= E')); eauto.
+             hnf; intros.  hnf in H8.  specialize (H8 x H6).
+             pose proof (crash_ssa_eval_agree L L' (stmtIf e sc t) (ann2 (D0, D') ans ant) s'  E' Es).
+             eapply H13; eauto; econstructor; eauto.
+           - rewrite H6.  rewrite condTrue.  intros; subst; eauto. }
+         { assert (exp_eval Es e = Some v).
+           - eapply (exp_eval_agree (E:= E')); eauto.
+             hnf; intros.  hnf in H8.  specialize (H8 x H6).
+             pose proof (crash_ssa_eval_agree L L' (stmtIf e sc t) (ann2 (D0, D') ans ant) s'  E' Es).
+             eapply H13; eauto; econstructor; eauto.
+           - rewrite H6.  rewrite condTrue.  intros; subst; eauto. }
+    + exploit (IHCrash L L' ant sc E' Es s'); eauto.
+      * intros. rewrite H15 in H5; simpl in *; eauto.
+      *  case_eq (undef e); intros; simpl; unfold evalSexp.
+         {  assert (exp_eval Es e = Some v).
+            - eapply (exp_eval_agree (E:= E')); eauto.
+              hnf; intros.  hnf in H8.  specialize (H8 x H6).
+              pose proof (crash_ssa_eval_agree L L' (stmtIf e s sc) (ann2 (D0, D') ans ant) s'  E' Es).
+              eapply H13; eauto; econstructor; eauto.
+            - rewrite H6.  rewrite condFalse. intros; subst; eauto. }
+         { assert (exp_eval Es e = Some v).
+           - eapply (exp_eval_agree (E:= E')); eauto.
+             hnf; intros.  hnf in H8.  specialize (H8 x H6).
+              pose proof (crash_ssa_eval_agree L L' (stmtIf e s sc) (ann2 (D0, D') ans ant) s'  E' Es).
+              eapply H13; eauto; econstructor; eauto.
+           - rewrite H6.  rewrite condFalse.  intros; subst; eauto. }
+    + isabsurd.
+Qed.
+
+(*
+*** Local Variables: ***
+*** coq-load-path: (("../" "Lvc")) ***
+*** End: ***
+*)
